

(70)

Integration:-

Unit-3

Integration of a mble function w.r.t. a measure μ :-Let $f: \Omega \rightarrow \overline{\mathbb{R}}$ be a measurable function.To define $\int_{\Omega} f d\mu$ where μ is a measure defined on (Ω, \mathcal{A}) .So let $(\Omega, \mathcal{A}, \mu)$ be a measure space.let $f: \Omega \rightarrow \overline{\mathbb{R}}$. We will define $\int_{\Omega} f d\mu$ when(i) f is non-ve simple function(ii) f is non-ve mble function(iii) f is any mble function.(i) Let f be a non-ve simple function.

$$\text{i.e. } f = \sum_{j=1}^n a_j I_{A_j}, \quad a_j \geq 0 \text{ \& distinct,}$$

$$A_i \cap A_j = \emptyset \quad \forall i \neq j \text{ \&}$$

$$\bigcup_{j=1}^n A_j = \Omega, \quad A_j \in \mathcal{A} \quad \forall j.$$

Def: Integral of a non-ve simple function $f = \sum_{j=1}^n a_j I_{A_j}$ is defined as

$$\int_{\Omega} f d\mu = \sum_{j=1}^n a_j \mu(A_j)$$

(ii) Let f be non-ve mble function.We know that if $f \geq 0$, mble, then $\exists \{f_n\}$ such that $f_n \geq 0$, f_n simple &

$$0 \leq f_n \uparrow f$$

then

Def

$$\int_{\Omega} f d\mu = \lim_{n \rightarrow \infty} \int_{\Omega} f_n d\mu$$

(71) let f be any mble function, then

Def $\int f du$ is said to exist, if

$$\int f^+ du < \infty \quad \text{or} \quad \int f^- du < \infty$$

and whenever it exists,

$$\int f du = \int f^+ du - \int f^- du$$

[check for existance is necessary first]

[Note: $\int f du$ does not exist if $\int f^\pm du = \infty$.

e.g. let $f(x) = \frac{1}{\pi} \frac{1}{1+x^2}$

$$\begin{aligned} \neq E(x) &= \int x f(x) dx = \frac{1}{\pi} \int_{-\infty}^{\infty} \frac{x}{1+x^2} dx \\ &= \frac{1}{\pi} \left[\int_{-\infty}^0 + \int_0^{\infty} \right] \end{aligned}$$

Thus $\int x f(x) dx$ does not exist.]

Def: A mble function f is said to be integrable if both $\int f^+ du$ and $\int f^- du$ are finite \neq then $\int f du < \infty$.

Remark: It is necessary to show that the definition of integrals are unambiguous.

Properties of integrals :-

$$\text{If } A \in \mathcal{A} \neq A \subset \mathbb{R} \text{ then } \int_A f du = \int f I_A du$$

Let $\int f du$, $\int g du$ \neq $\int f du$ + $\int g du$ exists.

(i.e either both finite or both $+\infty$ or $-\infty$ or one of them finite)

Then we have the following properties of integrals.

(72)

(A) Linearity property:-

$$(i) \int_{\Omega} (f+g) d\mu = \int_{\Omega} f d\mu + \int_{\Omega} g d\mu$$

$$(ii) \int_{A \cup B} f d\mu = \int_A f d\mu + \int_B f d\mu, \quad A, B \in \mathcal{A}, \quad A \cap B = \emptyset$$

$$(iii) \text{ For a constant } c, \int c f d\mu = c \int f d\mu$$

(B) Order preserving property.

$$(i) f \geq 0 \Rightarrow \int f d\mu \geq 0$$

$$(ii) f \geq g \Rightarrow \int f d\mu \geq \int g d\mu$$

$$(iii) f = g \text{ a.e.} \Rightarrow \int f d\mu = \int g d\mu$$

—X—

Step I : Establish Def. 1 is full proof

II : " properties A & B for non-ve simple function

Step III : " Def 2 is full proof

IV : " properties A & B for non-ve mble function

V : " Def 3 is full proof

VI : " properties A & B for any mble function

—X—

Step I : Let f be a non-ve simple function. Suppose we write

$$f = \sum_{i=1}^m a_i I_{A_i} \quad \& \quad f = \sum_{j=1}^n b_j I_{B_j}$$

$$\text{then } \int f d\mu = \sum_{i=1}^m a_i \mu(A_i) \quad \& \quad \text{also } \int f d\mu = \sum_{j=1}^n b_j \mu(B_j)$$

$$\text{To prove } \sum_{i=1}^m a_i \mu(A_i) = \sum_{j=1}^n b_j \mu(B_j)$$

Proof : Note $w \in A_i \cap B_j \Rightarrow a_i = b_j$

$$\begin{aligned} \text{Consider } \sum_{i=1}^m a_i \mu(A_i) &= \sum_{i=1}^m a_i \mu(A_i \cap \Omega) \\ &= \sum_{i=1}^m a_i \mu\left(A_i \cap \left(\bigcup_{j=1}^n B_j\right)\right) \end{aligned}$$

(73)

$$= \sum_{i=1}^m a_i \mu \left[\bigcup_{j=1}^n (A_i \cap B_j) \right]$$

$$= \sum_{i=1}^m a_i \sum_{j=1}^n \mu(A_i \cap B_j) \quad \because A_i \cap B_j \subset A_i$$

are disjoint sets.

$$= \sum_{i=1}^m \sum_{j=1}^n a_i \mu(A_i \cap B_j) \quad \text{--- (1)}$$

Similarly

$$\sum_{j=1}^n b_j \mu(B_j) = \sum_{j=1}^n \sum_{i=1}^m b_j \mu(A_i \cap B_j) \quad \text{--- (2)}$$

but $a_i = b_j$ on $A_i \cap B_j$

$$\Rightarrow \int f d\mu = \sum_{i=1}^m \sum_{j=1}^n a_i \mu(A_i \cap B_j) = \sum_{j=1}^n \sum_{i=1}^m b_j \mu(A_i \cap B_j)$$

$$\text{i.e. } \sum_{i=1}^m a_i \mu(A_i) = \sum_{j=1}^n b_j \mu(B_j)$$

Thus the definition of integral of a non-re
simple function is full proof.

—x—

Step II: A(i)

$$\text{To prove } \int (f+g) d\mu = \int f d\mu + \int g d\mu$$

$$\text{let } f = \sum_{i=1}^m a_i I_{A_i} \quad \& \quad \text{let } g = \sum_{j=1}^n b_j I_{B_j}$$

$$\text{then } f+g = \sum_{i=1}^m \sum_{j=1}^n (a_i + b_j) I_{A_i \cap B_j}$$

$$\begin{aligned} \therefore \int (f+g) d\mu &= \sum_{i=1}^m \sum_{j=1}^n (a_i + b_j) \mu(A_i \cap B_j) \\ &= \sum_{i=1}^m \sum_{j=1}^n a_i \mu(A_i \cap B_j) + \sum_{i=1}^m \sum_{j=1}^n b_j \mu(A_i \cap B_j) \\ &= \sum_{i=1}^m a_i \mu\left(A_i \cap \bigcup_{j=1}^n B_j\right) + \sum_{j=1}^n b_j \mu\left(\bigcup_{i=1}^m A_i \cap B_j\right) \\ &= \sum_{i=1}^m a_i \mu(A_i) + \sum_{j=1}^n b_j \mu(B_j) \\ &= \int f d\mu + \int g d\mu \end{aligned}$$

—x—

A(ii) To prove $\int_{A \cup B} f d\mu = \int_A f d\mu + \int_B f d\mu$

where $A \cap B = \emptyset$
Proof: $\int_{A \cup B} f d\mu = \int f I_{A \cup B} d\mu$, but $I_{A \cup B} = I_A + I_B$
 $\therefore A \cap B = \emptyset$.

$$\begin{aligned} \therefore \int_{A \cup B} f d\mu &= \int f (I_A + I_B) d\mu \\ &= \int f I_A d\mu + \int f I_B d\mu \\ &= \int_A f d\mu + \int_B f d\mu \end{aligned}$$

A(iii) Let C be a constant

To prove $\int C f d\mu = C \int f d\mu$

If $C=0$ then $Cf=0$ & hence both sides are zero.

If $C>0$ then $f = \sum_{i=1}^m a_i I_{A_i}$
 $(0 < C < \infty)$ $\therefore Cf = \sum_{i=1}^m (Ca_i) I_{A_i}$

$$\begin{aligned} \text{then } \int Cf d\mu &= \sum_{i=1}^m (Ca_i) \mu(A_i) \\ &= C \sum_{i=1}^m a_i \mu(A_i) \end{aligned}$$

$$= C \int f d\mu$$

(B)(i) To prove if $f \geq 0 \Rightarrow \int f d\mu \geq 0$

$f \geq 0 \Rightarrow$ all a_i 's ≥ 0 also μ is non-neg

$$\Rightarrow \int f d\mu = \sum_{i=1}^m a_i \mu(A_i) \geq 0$$

(ii) $f \geq g \Rightarrow \int f d\mu \geq \int g d\mu$

$$f \geq g \Rightarrow f - g \geq 0$$

$$\text{Now } f = f - g + g$$

$$\begin{aligned} \therefore \int f d\mu &= \int (f - g) d\mu + \int g d\mu \\ &\geq \int g d\mu \end{aligned}$$

(75) (iii) If $f = g$ a.e., then $\int f d\mu = \int g d\mu$

Let $A = \{f = g\}$ then $f = g$ a.e. $\Rightarrow \mu(A^c) = 0$

Now consider

$$\int (f - g) d\mu = \int_A (f - g) d\mu + \int_{A^c} (f - g) d\mu$$

$$= 0 + \int (f - g) \cdot \mathbb{I}_{A^c} d\mu$$

$$= 0 + 0 \quad \because A \cap B_j \cap A^c = \emptyset$$

$$\Rightarrow \int (f - g) d\mu = 0$$

$$\therefore \int f d\mu = \int (f - g + g) d\mu$$

$$= \int (f - g) d\mu + \int g d\mu$$

$$= \int g d\mu$$

hence proved.

→

Step III: TP Def. (2) is full proof.

We accept this result without proof.

(A part of proof is as follows).

[Result :- Let $\{X_n\}$ be a non-decreasing sequence of non-negative simple functions s.t. $X_n \rightarrow X$. Let $X \geq Y$, where Y is non-negative simple fⁿ then $\lim \int X_n d\mu \geq \int Y d\mu$]

Assuming the above result holds, we can prove Def. (2) is full proof or unambiguous.

Def 2: $0 \leq f_n \uparrow f$, f_n simple $\forall n$ then

$$\int f d\mu = \lim_n \int f_n d\mu$$

To prove this def is full proof, if possible,

suppose $0 \leq f_n \uparrow f$, f_n simple

$0 \leq g_n \uparrow f$, g_n simple

To prove $\lim_{n \rightarrow \infty} \int f_n d\mu = \lim_{n \rightarrow \infty} \int g_n d\mu$

(76) Note that \forall fixed $k \geq 1$,
 $f \geq g_k$, g_k simple

ii by above result,

$$\lim_{n \rightarrow \infty} \int f_n du \geq \int g_k du \quad \forall k \geq 1$$

let $k \rightarrow \infty$ then

$$\lim_{n \rightarrow \infty} \int f_n du \geq \lim_{k \rightarrow \infty} \int g_k du \quad \text{--- (1)}$$

On similar lines, we can prove that

$$\lim_{n \rightarrow \infty} \int g_n du \geq \lim_{m \rightarrow \infty} \int f_m du \quad \text{--- (2)}$$

From (1) & (2), we have

$$\lim_{n \rightarrow \infty} \int f_n du = \lim_{n \rightarrow \infty} \int g_n du$$

Thus $\int f du$ is unambiguously defined if $f \geq 0$.

Step IV: To prove properties of integral of non-negative f^n :-

$$A(i) \quad \int (f+g) du = \int f du + \int g du$$

where $f \neq g \geq 0$, mble f^n .

Recall $0 \leq f_n \uparrow f$, f_n simple, $0 \leq g_n \uparrow g$, g_n simple

then $0 \leq f_n + g_n \uparrow f + g$, $f_n + g_n$ simple

$$\begin{aligned} \text{ii} \quad \int (f+g) du &= \lim_{n \rightarrow \infty} \int (f_n + g_n) du \\ &= \lim_{n \rightarrow \infty} \left[\int f_n du + \int g_n du \right] \\ &= \lim_{n \rightarrow \infty} \int f_n du + \lim_{n \rightarrow \infty} \int g_n du \\ &= \int f du + \int g du \end{aligned}$$

hence proved.

$$A(ii) \quad \int_{A \cup B} f du = \int_A f du + \int_B f du, \quad A \cap B = \emptyset.$$

In fact, all properties A(ii), A(iii) & B(i), B(ii)

B(iii) hold for non-negative mble f^n .

(can be proved on similar lines as A(i))

(77) Def 3 : Integral of a mble f^n .
Step V: Let f be a mble function.
 $\int f d\mu$ is said to exist if $\int f^+ d\mu < \infty$ or $\int f^- d\mu < \infty$. Then $\int f d\mu = \int f^+ d\mu - \int f^- d\mu$
 This definition is unambiguous by itself, because $\int f^+ d\mu$ & $\int f^- d\mu$ are unambiguously defined.

Properties: Let f and g be any mble function s.t.

$\int f d\mu, \int g d\mu$ & $\int f d\mu + \int g d\mu$ exists.

$\int f d\mu$ can be $\pm\infty$, $\int g d\mu$ can be $\pm\infty$ but $\int f d\mu + \int g d\mu$ exists

$\Rightarrow \int f d\mu$ & $\int g d\mu$ both can be $+\infty$
 OR " " " " $-\infty$

but not one $+\infty$ & the other $-\infty$.

Then A (i) $\int (f+g) d\mu = \int f d\mu + \int g d\mu$

Proof: Define

$$A_1 = \{ \omega \mid f \geq 0, g \geq 0 \}$$

$$A_2 = \{ \omega \mid f \geq 0, g < 0, f+g \geq 0 \}$$

$$A_3 = \{ \omega \mid f \geq 0, g < 0, f+g < 0 \}$$

$$A_4 = \{ \omega \mid f < 0, g < 0, f+g < 0 \}$$

$$A_5 = \{ \omega \mid f < 0, g \geq 0, f+g \geq 0 \}$$

$$\& A_6 = \{ \omega \mid f < 0, g \geq 0, f+g < 0 \}$$

then $A_i \cap A_j = \emptyset \quad \forall i \neq j$ & $\bigcup_i A_i = \Omega$

We shall prove that

$$\int_{A_k} (f+g) d\mu = \int_{A_k} f d\mu + \int_{A_k} g d\mu, \quad k=1, 2, \dots, 6.$$

(78)

For set A_1 & A_4 i.e for $k=1$ & 4 , the result is obvious.

Suppose $k=2$

$$\text{write } f+g = f - (-g)$$

$$\text{i.e } f = f+g + (-g) \quad \text{on } A_2$$

Here f , $f+g$ & $-g$ all are non-negative mble f 's & hence

$$\begin{aligned} \int_{A_2} f du &= \int_{A_2} (f+g) du + \int_{A_2} -g du \\ &= \int_{A_2} (f+g) du - \int_{A_2} g du \end{aligned}$$

$$\text{i.e } \int_{A_2} (f+g) du = \int_{A_2} f du + \int_{A_2} g du$$

On similar lines, we can prove that-

$$\int_{A_k} (f+g) du = \int_{A_k} f du + \int_{A_k} g du \quad \text{for } k=3, 5, 6.$$

\therefore adding all such results, we have (& rearranging the terms)

$$\sum_{k=1}^6 \int_{A_k} (f+g) du = \sum_{k=1}^6 \int_{A_k} f du + \sum_{k=1}^6 \int_{A_k} g du$$

$$\Rightarrow \int_{\Omega} (f+g) du = \int_{\Omega} f du + \int_{\Omega} g du$$

On similar lines, we can prove the remaining properties

—x—
Integrability property :—

A mble f^n f is said to be integrable if

$$\int f^+ du < \infty \quad \& \quad \int f^- du < \infty$$

$$\text{In that case } \int f du = \int f^+ du - \int f^- du < \infty.$$

$$\text{Now } |f| = f^+ + f^-$$

$$\therefore \int |f| du = \int f^+ du + \int f^- du < \infty$$

Note that in general $\int |f| du$ always exists.

\therefore it is either $< \infty$ or $= +\infty$

(79) Thus

i) f is integrable iff $\int |f| du < \infty$.

ii) If $|f| \leq g$, g integrable
then f is integrable

Proof: $|f| \leq g \Rightarrow \int |f| du \leq \int g du < \infty$

$$\Rightarrow \int |f| du < \infty$$

$\Rightarrow f$ is integrable

iii) $f = g$ a.e. $\Rightarrow \int f du = \int g du$

Let $N = \{w \mid f \neq g\}$ then $N' = \{w \mid f \neq g\}^c$

Now $\mu(N') = 0$

$$\int f du = \int_N f du + \int_{N'} f du = \int_N f du$$

$$\text{Similarly } \int g du = \int_N g du + \int_{N'} g du = \int_N g du$$

$$\therefore \mu(N') = 0$$

$$\text{but on } N, f = g \Rightarrow \int_N f du = \int_N g du$$

$$\Rightarrow \int f du = \int g du$$

—x—

Remark: The 2nd definition uses sequence of non-re simple function $\{f_n\}$ s.t. $f_n \uparrow f$, then $\int f_n du \rightarrow \int f du$ where f is non-re mble fⁿ.

What will happen if $\{f_n\}$ is a seq. of non-re mble functions?

The answer is in the following famous theorem.

Convergence Theorem: